Effect-casting for derivations

Refinery/Signature.lean
@@ -12,13 +12,23 @@ class Signature (φ : Type _) (α : outParam (Type _)) (ε : outParam (Type _))
 
 variable {φ : Type _} {α : Type _} {ε : Type _} [Signature φ α ε]
 
+def Signature.HasEff (e : ε) (f : φ) := eff f ≤ e
+
+theorem Signature.HasEff.mono {e e' : ε} (he : e ≤ e') {f : φ} (h : HasEff e f) : HasEff e' f
+  := le_trans h he
+
 structure Signature.IsFn (f : φ) (e : ε) (A B : Ty α) where
   src : A = src f
   trg : B = trg f
-  eff : eff f ≤ e
+  eff : HasEff e f
 
-theorem Signature.IsFn.mono {f : φ} {e e' : ε} {A B : Ty α} (h : IsFn f e A B) (h' : e ≤ e')
-  : IsFn f e' A B := ⟨h.src, h.trg, le_trans h.eff h'⟩
+attribute [simp] Signature.IsFn.eff
+
+theorem Signature.IsFn.withEff {f : φ} {e e' : ε} {A B : Ty α} (h : IsFn f e A B) (he : HasEff e' f)
+  : IsFn f e' A B := ⟨h.src, h.trg, he⟩
+
+theorem Signature.IsFn.mono {f : φ} {e e' : ε} {A B : Ty α} (h : IsFn f e A B) (he : e ≤ e')
+  : IsFn f e' A B := ⟨h.src, h.trg, h.eff.mono he⟩
 
 theorem Signature.IsFn.top {f : φ} {e : ε} {A B : Ty α} (h : IsFn f e A B) : IsFn f ⊤ A B
   := h.mono le_top
