Refinery/Term/Extrinsic/Effect.lean
@@ -1,0 +1,135 @@
+import Refinery.Signature
+import Refinery.Term.Syntax
+
+namespace Refinery
+
+open HasQuant
+
+namespace Term
+
+variable {φ : Type u} {α : Type v} {ε : Type w} [S : Signature φ α ε]
+
+inductive HasEff : ε → Term φ (Ty α) → Prop
+  | bv (n) : HasEff e .(bv n)
+  | op {e f a} : S.HasEff e f → HasEff e a → HasEff e (.op f a)
+  | let₁ {e A a b} : HasEff e a → HasEff e b → HasEff e (.let₁ a A b)
+  | let₂ {e A B a b} : HasEff e a → HasEff e b → HasEff e (.let₂ a A B b)
+  | unit : HasEff e .unit
+  | pair {e a b} : HasEff e a → HasEff e b → HasEff e (.pair a b)
+  | inl {e A B a} : HasEff e a → HasEff e (.inl A B a)
+  | inr {e A B b} : HasEff e b → HasEff e (.inr A B b)
+  | case {e A B a b c} : HasEff e a → HasEff e b → HasEff e c → HasEff e (.case a A B b c)
+  | abort {e A a} : HasEff e a → HasEff e (.abort A a)
+  | iter {e A B a b} : e ∈ S.iterative → HasEff e a → HasEff e b → HasEff e (.iter a A B b)
+
+attribute [simp] HasEff.bv HasEff.unit
+
+syntax "inductive_and" : tactic
+
+macro_rules
+  | `(tactic| inductive_and) => `(tactic| {
+    apply Iff.intro
+    · intro h; cases h; (repeat first | assumption | constructor)
+    · intro h; (try casesm* _ ∧ _); constructor <;> assumption
+  })
+
+@[simp]
+theorem HasEff.op_iff {e : ε} {f : φ} {a : Term φ (Ty α)}
+  : HasEff e (.op f a) ↔ S.HasEff e f ∧ HasEff e a := by inductive_and
+
+theorem HasEff.op_fn {e : ε} {f : φ} {a : Term φ (Ty α)} (h : HasEff e (.op f a))
+  : S.HasEff e f := by rw [HasEff.op_iff] at h; exact h.1
+
+theorem HasEff.op_arg {e : ε} {f : φ} {a : Term φ (Ty α)} (h : HasEff e (.op f a))
+  : HasEff e a := by rw [HasEff.op_iff] at h; exact h.2
+
+@[simp]
+theorem HasEff.let₁_iff {e : ε} {A : Ty α} {a b : Term φ (Ty α)}
+  : HasEff e (.let₁ a A b) ↔ HasEff e a ∧ HasEff e b := by inductive_and
+
+theorem HasEff.let₁_bind {e : ε} {A : Ty α} {a b : Term φ (Ty α)} (h : HasEff e (.let₁ a A b))
+  : HasEff e a := by rw [HasEff.let₁_iff] at h; exact h.1
+
+theorem HasEff.let₁_body {e : ε} {A : Ty α} {a b : Term φ (Ty α)} (h : HasEff e (.let₁ a A b))
+  : HasEff e b := by rw [HasEff.let₁_iff] at h; exact h.2
+
+@[simp]
+theorem HasEff.let₂_iff {e : ε} {A B : Ty α} {a b : Term φ (Ty α)}
+  : HasEff e (.let₂ a A B b) ↔ HasEff e a ∧ HasEff e b := by inductive_and
+
+theorem HasEff.let₂_bind {e : ε} {A B : Ty α} {a b : Term φ (Ty α)} (h : HasEff e (.let₂ a A B b))
+  : HasEff e a := by rw [HasEff.let₂_iff] at h; exact h.1
+
+theorem HasEff.let₂_body {e : ε} {A B : Ty α} {a b : Term φ (Ty α)} (h : HasEff e (.let₂ a A B b))
+  : HasEff e b := by rw [HasEff.let₂_iff] at h; exact h.2
+
+@[simp]
+theorem HasEff.pair_iff {e : ε} {a b : Term φ (Ty α)}
+  : HasEff e (.pair a b) ↔ HasEff e a ∧ HasEff e b := by inductive_and
+
+theorem HasEff.pair_fst {e : ε} {a b : Term φ (Ty α)} (h : HasEff e (.pair a b))
+  : HasEff e a := by rw [HasEff.pair_iff] at h; exact h.1
+
+theorem HasEff.pair_snd {e : ε} {a b : Term φ (Ty α)} (h : HasEff e (.pair a b))
+  : HasEff e b := by rw [HasEff.pair_iff] at h; exact h.2
+
+@[simp]
+theorem HasEff.inl_iff {e : ε} {A B : Ty α} {a : Term φ (Ty α)}
+  : HasEff e (.inl A B a) ↔ HasEff e a := by inductive_and
+
+theorem HasEff.inl_arg {e : ε} {A B : Ty α} {a : Term φ (Ty α)} (h : HasEff e (.inl A B a))
+  : HasEff e a := by rw [HasEff.inl_iff] at h; exact h
+
+@[simp]
+theorem HasEff.inr_iff {e : ε} {A B : Ty α} {b : Term φ (Ty α)}
+  : HasEff e (.inr A B b) ↔ HasEff e b := by inductive_and
+
+theorem HasEff.inr_arg {e : ε} {A B : Ty α} {b : Term φ (Ty α)} (h : HasEff e (.inr A B b))
+  : HasEff e b := by rw [HasEff.inr_iff] at h; exact h
+
+@[simp]
+theorem HasEff.case_iff {e : ε} {A B : Ty α} {a b c : Term φ (Ty α)}
+  : HasEff e (.case a A B b c) ↔ HasEff e a ∧ HasEff e b ∧ HasEff e c := by inductive_and
+
+theorem HasEff.case_desc {e : ε} {A B : Ty α} {a b c : Term φ (Ty α)}
+  (h : HasEff e (.case a A B b c))
+  : HasEff e a := by rw [HasEff.case_iff] at h; exact h.1
+
+theorem HasEff.case_left {e : ε} {A B : Ty α} {a b c : Term φ (Ty α)}
+  (h : HasEff e (.case a A B b c))
+  : HasEff e b := by rw [HasEff.case_iff] at h; exact h.2.1
+
+theorem HasEff.case_right {e : ε} {A B : Ty α} {a b c : Term φ (Ty α)}
+  (h : HasEff e (.case a A B b c))
+  : HasEff e c := by rw [HasEff.case_iff] at h; exact h.2.2
+
+@[simp]
+theorem HasEff.abort_iff {e : ε} {A : Ty α} {a : Term φ (Ty α)}
+  : HasEff e (.abort A a) ↔ HasEff e a := by inductive_and
+
+theorem HasEff.abort_arg {e : ε} {A : Ty α} {a : Term φ (Ty α)} (h : HasEff e (.abort A a))
+  : HasEff e a := by rw [HasEff.abort_iff] at h; exact h
+
+@[simp]
+theorem HasEff.iter_iff {e : ε} {A B : Ty α} {a b : Term φ (Ty α)}
+  : HasEff e (.iter a A B b) ↔ e ∈ S.iterative ∧ HasEff e a ∧ HasEff e b := by inductive_and
+
+theorem HasEff.iter_eff {e : ε} {A B : Ty α} {a b : Term φ (Ty α)} (h : HasEff e (.iter a A B b))
+  : e ∈ S.iterative := by rw [HasEff.iter_iff] at h; exact h.1
+
+theorem HasEff.iter_init {e : ε} {A B : Ty α} {a b : Term φ (Ty α)} (h : HasEff e (.iter a A B b))
+  : HasEff e a := by rw [HasEff.iter_iff] at h; exact h.2.1
+
+theorem HasEff.iter_body {e : ε} {A B : Ty α} {a b : Term φ (Ty α)} (h : HasEff e (.iter a A B b))
+  : HasEff e b := by rw [HasEff.iter_iff] at h; exact h.2.2
+
+@[simp]
+theorem HasEff.wk_iff (ρ : ℕ → ℕ) {e : ε} {a : Term φ (Ty α)} : HasEff e (a.ren ρ) ↔ HasEff e a :=
+  by induction a generalizing ρ <;> simp [*]
+
+theorem HasEff.mono {e e' : ε} (he : e ≤ e') {a : Term φ (Ty α)} (h : HasEff e a) : HasEff e' a :=
+  by induction h <;> simp [Signature.HasEff.mono he, S.iterative_is_upper he, *]
+
+end Term
+
+end Refinery
